case_study/RiscvPmp/IrisInstance.v
@@ -30,7 +30,6 @@ From Katamaran Require Import
      Base
      Hoare
      Bitvector
-     trace
      Iris.Instance
      Iris.Base
      Syntax.Predicates
@@ -38,6 +37,7 @@ From Katamaran Require Import
      RiscvPmp.PmpCheck
      RiscvPmp.Machine
      RiscvPmp.IrisModel
+     RiscvPmp.trace
      RiscvPmp.Sig.
 
 From iris.base_logic Require Import invariants lib.iprop lib.gen_heap.
@@ -107,8 +107,8 @@ Module RiscvPmpIrisAdeqParameters <: IrisAdeqParameters RiscvPmpBase RiscvPmpIri
         now rewrite map_map map_id.
   Qed.
 
-  Lemma mem_inv_init `{gHP : !mcMemPreGS Σ} (μ : Memory) :
-    ⊢ |==> ∃ mG : mcMemGS Σ, (mem_inv mG μ ∗ mem_res μ)%I.
+  Lemma mem_init `{gHP : !mcMemPreGS Σ} (μ : Memory) :
+    ⊢ |==> ∃ mG : mcMemGS Σ, (mem_state_interp mG μ ∗ mem_res μ)%I.
   Proof.
     pose (memmap := initMemMap μ).
     iMod (gen_heap_init (L := Addr) (V := MemVal) memmap) as (gH) "[Hinv [Hmapsto _]]".
@@ -443,7 +443,10 @@ Module RiscvPmpIrisInstance (FL : FailLogic) <:
 
     Import env.notations.
 
-    Equations(noeqns) luser_inst `{sailRegGS Σ, invGS Σ, mcMemGS Σ}
+    (* We don't need additional ghost state beyond what we already have for the WP. *)
+    Definition resGS := trivGS.
+
+    Equations(noeqns) luser_inst `{sailRegGS Σ, invGS Σ, mcMemGS Σ, trivGS Σ}
       (p : Predicate) (ts : Env Val (𝑯_Ty p)) : iProp Σ :=
     | pmp_entries              | [ v ]                => interp_pmp_entries v
     | pmp_addr_access          | [ entries; m ]       => interp_pmp_addr_access liveAddrs mmioAddrs entries m
@@ -468,7 +471,7 @@ Module RiscvPmpIrisInstance (FL : FailLogic) <:
           destruct x; auto
       end.
 
-    Definition lduplicate_inst `{sailRegGS Σ, invGS Σ, mcMemGS Σ} :
+    Definition lduplicate_inst `{sailRegGS Σ, invGS Σ, mcMemGS Σ, trivGS Σ} :
       forall (p : Predicate) (ts : Env Val (𝑯_Ty p)),
         is_duplicable p = true ->
         (luser_inst p ts) ⊢ (luser_inst p ts ∗ luser_inst p ts).
